Notion of "solved"

Abstract_Formula.thy
@@ -10,6 +10,7 @@ begin
 lift_definition fset_from_list :: "'a list => 'a fset" is set by (rule finite_set)
 lemma mem_fset_from_list[simp]: "x |\<in>| fset_from_list l  \<longleftrightarrow> x \<in> set l" by transfer rule
 lemma fimage_fset_from_list[simp]: "f |`| fset_from_list l = fset_from_list (map f l)"  by transfer auto
+lemma fset_fset_from_list[simp]: "fset (fset_from_list l) = set l"  by transfer auto
 end
 
 
@@ -19,8 +20,10 @@ locale Abstract_Formulas =
   fixes fv :: "'form \<Rightarrow> ('var \<times> 'annot) set"
   fixes subst :: "'subst \<Rightarrow> 'form \<Rightarrow> 'form"
   fixes ran_fv :: "'subst \<Rightarrow> ('var \<times> 'annot) set"
+  fixes closed :: "'preform \<Rightarrow> bool"
   assumes annotate_preserves_fv: "fst ` fv (annotate a pf) = pre_fv pf"
   assumes fv_subst: "fv (subst s f) \<subseteq> ran_fv s"
+  assumes closed_eq: "closed pf \<Longrightarrow> subst s1 (annotate a1 pf) = subst s2 (annotate a2 pf)"
 
 locale Abstract_Rules =
   Abstract_Formulas _ pre_fv _ subst
@@ -36,11 +39,26 @@ begin
 end
 
 locale Abstract_Task =
-  Abstract_Rules  _ _ _ pre_fv _ _ _ rules
+  Abstract_Rules  _ _ _ _ pre_fv _ _ _ rules
   for rules :: "'rule stream" and pre_fv :: "'preform \<Rightarrow> 'var set" + 
   fixes assumptions :: "'preform list"
   fixes conclusions :: "'preform list"
+  assumes assumptions_closed: "\<forall>a \<in> set assumptions. closed a"
+  assumes conclusions_closed: "\<forall>c \<in> set conclusions. closed a"
   assumes no_empty_conclusions: "\<forall>xs\<in>sset rules. consequent xs \<noteq> []"
+begin
+  definition ass_forms where "ass_forms = fset_from_list (map (subst undefined) (map (annotate undefined) assumptions))"
+  definition conc_forms where "conc_forms = fset_from_list (map (subst undefined) (map (annotate undefined) conclusions))"
 
+  lemma subst_annotate_in_ass_formsI:
+    assumes "pf \<in> set assumptions"
+    shows "subst s (annotate a pf) |\<in>| ass_forms"
+      using assms ass_forms_def assumptions_closed closed_eq by fastforce
+
+  lemma subst_annotate_in_conc_formsI:
+    assumes "pf \<in> set conclusions"
+    shows "subst s (annotate a pf) |\<in>| conc_forms"
+      using assms conc_forms_def conclusions_closed closed_eq by fastforce
+end
 
 end
