Incredible_Correctness.thy
@@ -47,6 +47,12 @@ inductive_set global_assms where
 inductive_set local_assms for v p pth t where
   "(v',p') \<in> insert (v,p) (snd ` set pth) \<Longrightarrow> h |\<in>| hyps_for (nodeOf v') p' \<Longrightarrow> labelAtOut v' h \<in> local_assms v p pth t"
 
+lemma local_assms_Nil:
+  "local_assms v' a [] t = labelAtOut v' ` fset (hyps_for (nodeOf v') a)"
+  apply (auto 4 4 simp add: local_assms.simps )
+  apply (metis surjective_pairing)
+  done
+
 lemma local_assms_cons:
   "local_assms v' a (((v', p'), (v, p))#pth) t = labelAtOut v' ` fset (hyps_for (nodeOf v') a) \<union> local_assms v p pth t"
   apply (auto 4 4 simp add: local_assms.simps )
@@ -64,8 +70,14 @@ lemma out_port_cases[consumes 1, case_names Assumption Hyp Rule]:
     | r f where "n = Rule r" and "p = Reg f"
   using assms by (atomize_elim, cases p; cases n) auto
 
+lemma hyps_for_fimage: "hyps_for (Rule r) x = (if x |\<in>| f_antecedent r then (\<lambda> f. Hyp f x) |`| (fst x) else {||})"
+  apply (rule fset_eqI)
+  apply (rename_tac p')
+  apply (case_tac p')
+  apply (auto simp add:  split: if_splits out_port.splits)
+  done
   
-theorem correctness:
+theorem wf_tree:
   assumes "v |\<in>| vertices"
   assumes "p |\<in>| inPorts (nodeOf v)"
   assumes "global_assms \<subseteq> fset \<Gamma>"
@@ -139,24 +151,15 @@ case (wf \<Gamma> v p pth)
     with `nodeOf v' \<in> sset nodes`
     have "r \<in> sset rules"
       by (auto simp add: nodes_def stream.set_map)
-    moreover
+    
 
     from Rule  `p' |\<in>| outPorts (nodeOf v')`
     have "f |\<in>| f_consequent r" by simp
+    hence "f \<in> set (consequent r)" by (simp add: f_consequent_def)
+    with `r \<in> sset rules`
+    have "NatRule (r, f) \<in> sset (smap NatRule n_rules)"
+      by (auto simp add: stream.set_map n_rules_def no_empty_conclusions)
     moreover
-
-    {
-      fix x p h
-      assume 1: "x |\<in>| f_antecedent r"
-      have "hyps_for (nodeOf v') x = (\<lambda> f. Hyp f x) |`| (fst x)"
-        apply (rule fset_eqI)
-        apply (rename_tac p')
-        apply (case_tac p')
-        using 1
-        apply (auto simp add: Rule split: if_splits)
-        done
-    }
-    note * = this
 
     {
     from `f |\<in>| f_consequent r`
@@ -169,10 +172,10 @@ case (wf \<Gamma> v p pth)
     also
     have "subst (inst v') (annotate v' f) = labelAtOut v' p'" using Rule by (simp add: labelAtOut_def)
     also
-    note s
+    note `labelAtOut v' p' = labelAtIn v p`
     also
     have "?ant = ((\<lambda>x. (extra_assms v' x, labelAtIn  v' x)) |`| f_antecedent r)"
-      by (rule fimage_cong[OF refl])(auto simp add: labelAtIn_def labelAtOut_def *)
+      by (rule fimage_cong[OF refl]) (auto simp add: labelAtIn_def labelAtOut_def Rule hyps_for_fimage)
     also
     from effNatRuleI[OF calculation, where ctxt = \<Gamma>]
     have "eff (NatRule (r, f)) (\<Gamma>, labelAtIn v p) ((\<lambda>x. (extra_assms v' x |\<union>| \<Gamma>, labelAtIn  v' x)) |`| f_antecedent r)"
@@ -214,18 +217,55 @@ case (wf \<Gamma> v p pth)
       have "\<exists>\<Gamma> v p pth. x = tree \<Gamma> v p \<and> v |\<in>| vertices \<and> p |\<in>| inPorts (nodeOf v) \<and>  global_assms \<subseteq> fset \<Gamma> \<and> terminal_vertex t \<and> path v t pth \<and> local_assms v p pth t \<subseteq> fset \<Gamma>"
         by blast
     }
-    moreover
-
-    from `f |\<in>| _`
-    have "f \<in> set (consequent r)" by (simp add: f_consequent_def)
-    with `r \<in> sset rules`
-    have "NatRule (r, f) \<in> sset (smap NatRule n_rules)"
-      by (auto simp add: stream.set_map n_rules_def no_empty_conclusions)
     ultimately
 
     show ?thesis using Rule
       by (auto intro!: exI[where x = ?t]  simp add: comp_def   simp del: eff.simps)       
   qed
+qed
+
+lemma solved
+unfolding solved_def
+proof(intro ballI allI conjI impI)
+  fix c
+  assume "c |\<in>| conc_forms"
+  then obtain pf where "pf \<in> set conclusions" and "c = subst undefined (annotate undefined pf)"
+    by (auto simp add: conc_forms_def)
+  from this(1) conclusions_present
+  obtain v where "v |\<in>| vertices " and "nodeOf v = Conclusion pf"
+    by (auto, metis (no_types, lifting) image_iff image_subset_iff notin_fset)
+
+  let ?t = "tree ass_forms v ({||}, pf)"
+
+  have "wf ?t"
+  proof(rule wf_tree)
+    show "v |\<in>| vertices" by fact
+    show "({||}, pf) |\<in>| inPorts (nodeOf v)" using `nodeOf _ = _ `  by simp
+    show "global_assms \<subseteq> fset ass_forms"
+    proof
+      fix x
+      assume "x \<in> global_assms"
+      then obtain v pf where "v |\<in>| vertices" and "nodeOf v = Assumption pf" and "x = labelAtOut v (Reg pf)"
+        by (auto simp add: global_assms.simps)
+      from this (1,2) valid_nodes
+      have "Assumption pf \<in> sset nodes" by (auto simp add: fmember.rep_eq)
+      hence "pf \<in> set assumptions" by (auto simp add: nodes_def stream.set_map)
+      hence "closed pf" using assumptions_closed by auto
+      with `x = labelAtOut v (Reg pf)`
+      have "x = subst undefined (annotate undefined pf)" by (auto simp add: closed_eq labelAtOut_def)
+      thus "x \<in> fset ass_forms" using `pf \<in> set assumptions` by (auto simp add: ass_forms_def)
+    qed
+    show "terminal_vertex v" using `nodeOf v = Conclusion pf` by auto
+    show "path v v []"..
+    show "local_assms v ({||}, pf) [] v \<subseteq> fset ass_forms"
+      using `nodeOf v = Conclusion pf` by (auto simp add: local_assms_Nil)
+  qed
+  moreover
+  have "fst (root ?t) = (ass_forms, c)"
+    using `pf \<in> set conclusions` `c = _`
+    by (simp add: labelAtIn_def closed_eq conclusions_closed)
+  ultimately
+  show "\<exists>t. wf  t \<and> fst (root t) = (ass_forms, c)" by blast
 qed
 
 end
